progress on semaphore

rocq-brick-libcpp/proof/semaphore/inc.hpp
@@ -1,1 +1,4 @@
+// #define _LIBCPP_HAS_NO_THREADS
+// Paolo: /opt/homebrew/Cellar/llvm@19/19.1.7/include/c++/v1/semaphore
+#define __cpp_lib_atomic_wait
 #include <semaphore>
