rocq-brick-libcpp/proof/semaphore/test.cpp
@@ -3,7 +3,7 @@
 using namespace std;
 
 void test() {
-	std::binary_semaphore m{0};
+	std::binary_semaphore m{1};
   m.acquire();
   m.release();
 }
